<h2>Logical Equivalence</h2>
<p>Two propositions are equivalent if they always have the same truth value. Below is a truth table showing that the conditional <strong>p → q</strong> is equivalent to the contrapositive <strong>¬q → ¬p</strong>:</p>

<table class="truth-table">
    <tr>
        <th>p</th>
        <th>q</th>
        <th>¬p</th>
        <th>¬q</th>
        <th>p → q</th>
        <th>¬q → ¬p</th>
    </tr>
    <tr><td>T</td><td>T</td><td>F</td><td>F</td><td>T</td><td>T</td></tr>
    <tr><td>T</td><td>F</td><td>F</td><td>T</td><td>F</td><td>F</td></tr>
    <tr><td>F</td><td>T</td><td>T</td><td>F</td><td>T</td><td>T</td></tr>
    <tr><td>F</td><td>F</td><td>T</td><td>T</td><td>T</td><td>T</td></tr>
</table>

<p>Using a truth table to show non-equivalence:</p>
<!-- You can insert another table here for a non-equivalence example if needed -->
